Add Uncurry
This pass uncurries all applied lambdas.  Care is taken to not do beta
reduction and to not introduce spurious `Abs` or `App` nodes.

src/Experiments/SimplyTypedArithmetic.v
@@ -2699,6 +2699,12 @@ Module Compilers.
          | _ => None
          end.
 
+    Definition invert_or_expand_Pair {A B} (e : @expr var (type.prod A B)) : @expr var A * @expr var B
+      := match invert_Pair e with
+         | Some p => p
+         | None => (ident.fst @@ e, ident.snd @@ e)
+         end%core%expr.
+
     (* if we want more code for the below, I would suggest [reify_base_type] and [reflect_base_type] *)
     Definition reify_primitive {t} (v : type.interp (type.type_primitive t)) : @expr var (type.type_primitive t)
       := AppIdent (ident.primitive v) TT.
@@ -2838,6 +2844,189 @@ Module Compilers.
     Notation Reify v
       := (Reify_as (type.reify_type_of v) (fun _ => v)) (only parsing).
   End GallinaReify.
+
+  Module Uncurry.
+    Module type.
+      Fixpoint uncurried_domain (t : type) : type
+        := match t with
+           | type.arrow s d
+             => match d with
+                | type.arrow _ _
+                  => s * uncurried_domain d
+                | _ => s
+                end
+           | _ => type.type_primitive type.unit
+           end%ctype.
+
+      Definition uncurry (t : type) : type
+        := type.arrow (uncurried_domain t) (type.final_codomain t).
+
+      Section with_var.
+        Context (var : type -> Type).
+        Fixpoint value (t : type)
+          := match t with
+             | type.arrow s d
+               => value s -> value d
+             | t => @expr var t
+             end.
+      End with_var.
+    End type.
+
+    Fixpoint app_curried {t : type}
+      : type.interp t -> type.interp (type.uncurried_domain t) -> type.interp (type.final_codomain t)
+      := match t return type.interp t -> type.interp (type.uncurried_domain t) -> type.interp (type.final_codomain t) with
+         | type.arrow s d
+           => match d
+                    return (type.interp d -> type.interp (type.uncurried_domain d) -> type.interp (type.final_codomain d))
+                           -> type.interp (type.arrow s d)
+                           -> type.interp (type.uncurried_domain (type.arrow s d))
+                           -> type.interp (type.final_codomain d)
+              with
+              | type.arrow _ _ as d
+                => fun app_curried_d
+                       (f : type.interp s -> type.interp d)
+                       (x : type.interp s * type.interp (type.uncurried_domain d))
+                   => app_curried_d (f (fst x)) (snd x)
+              | d
+                => fun _
+                       (f : type.interp s -> type.interp d)
+                       (x : type.interp s)
+                   => f x
+              end (@app_curried d)
+         | _ => fun f _ => f
+         end.
+
+    Module expr.
+      Section reify_reflect.
+        Context {var : type -> Type}.
+        Fixpoint reify {t}
+          : type.value var t -> @expr var t
+          := match t with
+             | type.arrow s d
+               => fun f => Abs (fun v => @reify d (f (@reflect s (Var v))))
+             | _
+               => fun e => e
+             end%expr
+        with reflect {t}
+             : @expr var t -> type.value var t
+          := match t with
+             | type.arrow s d
+               => fun e (v : type.value _ s) => @reflect d (e @ (@reify s v))
+             | _
+               => fun e => e
+             end%expr.
+      End reify_reflect.
+
+      Section with_var.
+        Context {var : type -> Type}.
+
+        Definition reassociate_uncurried_domain_r_to_l {s s' d'}
+          : @expr var (type.uncurried_domain (s -> s' -> d'))
+            -> @expr var (type.uncurried_domain (s * s' -> d'))
+          := match d'
+                   return (expr (type.uncurried_domain (s -> s' -> d'))
+                           -> expr (type.uncurried_domain (s * s' -> d')))
+             with
+             | type.arrow _ _ as d'
+               => fun (e : expr (s * (s' * type.uncurried_domain d')))
+                  => let '(e, e') := invert_or_expand_Pair e in
+                     let '(e', e'') := invert_or_expand_Pair e' in
+                     (e, e', e'')%expr
+             | _
+               => fun e => e
+             end%core%expr.
+
+        Definition reassociate_uncurried_domain_l_to_r {s s' d'}
+          : @expr var (type.uncurried_domain (s * s' -> d'))
+            -> @expr var (type.uncurried_domain (s -> s' -> d'))
+          := match d'
+                   return (expr (type.uncurried_domain (s * s' -> d'))
+                           -> expr (type.uncurried_domain (s -> s' -> d')))
+             with
+             | type.arrow _ _ as d'
+               => fun (e : expr ((s * s') * type.uncurried_domain d'))
+                  => let '(e, e'') := invert_or_expand_Pair e in
+                     let '(e, e') := invert_or_expand_Pair e in
+                     (e, (e', e''))%expr
+             | _
+               => fun e => e
+             end%core%expr.
+
+        Fixpoint uncurried_abs {s d}
+          : (type.value var s -> type.value var d)
+            -> @expr var (type.uncurried_domain (type.arrow s d))
+            -> @expr var (type.final_codomain d)
+          := match d with
+             | type.arrow s' d'
+               => fun f x
+                  => @uncurried_abs
+                       (s * s')%ctype d'
+                       (fun xy
+                        => let '(x, y) := invert_or_expand_Pair xy in
+                           f (reflect x) (reflect y))
+                       (reassociate_uncurried_domain_r_to_l x)
+             | _
+               => fun f x => f (reflect x)
+             end%core%expr.
+
+        Fixpoint uncurried_app_to_value {s d}
+          : (@expr var (type.uncurried_domain (type.arrow s d))
+             -> @expr var (type.final_codomain d))
+            -> type.value var s
+            -> type.value var d
+          := match d with
+             | type.arrow s' d'
+               => fun f x (y : type.value var s')
+                  => @uncurried_app_to_value
+                       (s * s')%ctype d'
+                       (fun x' => f (reassociate_uncurried_domain_l_to_r x'))
+                       (reify x, reify y)
+             | _
+               => fun f x
+                  => f (reify x)
+             end%expr.
+
+        Definition uncurry_value {s d} (f : type.value var (s -> d))
+                   (x : type.value var s)
+          : type.value var d
+          := uncurried_app_to_value
+               (fun x' => Abs (fun v => uncurried_abs f (Var v)) @ x')%expr
+               x.
+
+        (** N.B. We only uncurry things when we hit an application of
+                 a lambda; everything else is untouched. *)
+        Fixpoint uncurry' {t} (e : @expr (type.value var) t) : type.value var t
+          := match e in expr.expr t return type.value var t with
+             | Var t v => v
+             | TT => TT
+             | AppIdent s d idc args
+               => reflect (AppIdent idc (reify (@uncurry' _ args)))
+             | App s d f x
+               => let f' := @uncurry' _ f in
+                  let x' := @uncurry' _ x in
+                  match invert_Abs f with
+                  | Some _ => uncurry_value f' x'
+                  | None => f' x'
+                  end
+             | Pair A B a b
+               => Pair (reify (@uncurry' A a)) (reify (@uncurry' B b))
+             | Abs s d f
+               => fun v : type.value var s => @uncurry' d (f v)
+             end.
+
+        Definition uncurry {t} (e : @expr (type.value var) t)
+          : @expr var (type.uncurry t)
+          := Abs (fun v : var (type.uncurried_domain t)
+                  => match t return type.value var t -> expr (type.uncurried_domain t) -> expr (type.final_codomain t) with
+                     | type.arrow _ _ => uncurried_abs
+                     | _ => fun e _ => e
+                     end (uncurry' e) (Var v)).
+      End with_var.
+
+      Definition Uncurry {t} (e : Expr t) : Expr (type.uncurry t)
+        := fun var => uncurry (e _).
+    End expr.
+  End Uncurry.
 
   Module CPS.
     Import Uncurried.
@@ -5835,6 +6024,48 @@ Module test9.
     exact I.
   Qed.
 End test9.
+Module test10.
+  Example test10 : True.
+  Proof.
+    let v := Reify (fun (f : Z -> Z -> Z) x y => f (x + y) (x * y))%Z in
+    pose v as E.
+    vm_compute in E.
+    pose (Uncurry.expr.Uncurry (PartialEvaluate true (canonicalize_list_recursion E))) as E'.
+    lazy in E'.
+    clear E.
+    lazymatch (eval cbv delta [E'] in E') with
+    | (fun var =>
+         (λ v,
+          ident.fst @@ Var v @
+                    (ident.fst @@ (ident.snd @@ Var v) + ident.snd @@ (ident.snd @@ Var v)) @
+                    (ident.fst @@ (ident.snd @@ Var v) * ident.snd @@ (ident.snd @@ Var v)))%expr)
+      => idtac
+    end.
+    constructor.
+  Qed.
+End test10.
+Module test11.
+  Example test11 : True.
+  Proof.
+    let v := Reify (fun x y => (fun f a b => f a b) (fun a b => a + b) (x + y) (x * y))%Z in
+    pose v as E.
+    vm_compute in E.
+    pose (Uncurry.expr.Uncurry (canonicalize_list_recursion E)) as E'.
+    lazy in E'.
+    clear E.
+    lazymatch (eval cbv delta [E'] in E') with
+    | (fun var =>
+        (λ v,
+         (λ v0,
+          ident.fst @@ Var v0 @ (ident.fst @@ (ident.snd @@ Var v0)) @
+          (ident.snd @@ (ident.snd @@ Var v0))) @
+         ((λ v0' v1, Var v0' + Var v1),
+          (ident.fst @@ Var v + ident.snd @@ Var v, ident.fst @@ Var v * ident.snd @@ Var v)))%expr)
+      => idtac
+    end.
+    constructor.
+  Qed.
+End test11.
 Axiom admit_pf : False.
 Notation admit := (match admit_pf with end).
 Ltac cache_reify _ :=
